Trochę walki z productivity checkerem, ale chyba przegranej.

code/BeatingProductivityChecker.v
@@ -1,5 +1,7 @@
 (** * F3v2: Liczby konaturalne [TODO] *)
 
+Require Import Coq.Program.Equality.
+
 Set Primitive Projections.
 
 Set Warnings "+cannot-define-projection".
@@ -40,7 +42,7 @@ Proof.
   - now constructor.
   - constructor.
     now apply CH.
-Qed.
+Defined.
 (* end hide *)
 
 Lemma sim_sym :
@@ -53,7 +55,7 @@ Proof.
   - now constructor.
   - constructor.
     now apply CH.
-Qed.
+Defined.
 (* end hide *)
 
 Lemma sim_trans :
@@ -68,7 +70,7 @@ Proof.
   - now constructor.
   - constructor.
     now apply CH with n2; [| congruence].
-Qed.
+Defined.
 (* end hide *)
 
 Inductive simBigF (R : conat -> conat -> Prop) : NatF conat -> NatF conat -> Prop :=
@@ -87,12 +89,74 @@ Lemma sim_to_simBig :
   forall n m : conat,
     sim n m -> simBig n m.
 Proof.
+  cofix CH.
   intros n m H.
   constructor.
   destruct H as [[]].
   - now constructor.
   - now constructor.
+Defined.
+
+Lemma simBig_to_sim :
+  forall n m : conat, 
+    simBig n m -> sim n m.
+Proof.
+  intros n m H.
+  constructor.
+  destruct H as [H].
+  induction H.
+  - now constructor.
+  - now apply (sim_refl {| out := n0 |}).
+  - destruct (sim_sym {| out := m0 |} {| out := n0 |}); [| easy].
+    now constructor; cbn.
+  - now destruct (sim_trans {| out := n1 |} {| out := n2 |} {| out := n3 |}).
 Qed.
+
+Module wut.
+
+Inductive simBigF (R : conat -> conat -> Prop) : NatF conat -> NatF conat -> Prop :=
+(* | simBigF_sim : forall n1 n2 : NatF conat, sim {| out := n1 |} {| out := n2 |} -> simBigF R n1 n2 *)
+| simBigF_Z : simBigF R Z Z
+| simBigF_S : forall n1 n2 : conat, R n1 n2 -> simBigF R (S n1) (S n2)
+(* | simBigF_refl : forall n : NatF conat, simBigF R n n *)
+| simBigF_sym : forall n m : NatF conat, simBigF R m n -> simBigF R n m
+| simBigF_trans :
+    forall (n1 n2 n3 : NatF conat), simBigF R n1 n2 -> simBigF R n2 n3 -> simBigF R n1 n3.
+
+CoInductive simBig (n m : conat) : Prop :=
+{
+  simBig' : simBigF simBig (out n) (out m);
+}.
+
+Lemma sim_to_simBig :
+  forall n m : conat,
+    sim n m -> simBig n m.
+Proof.
+  cofix CH.
+  intros n m H.
+  constructor.
+  destruct H as [[]].
+  - now constructor.
+  - constructor.
+    now apply CH.
+Defined.
+
+Lemma wut :
+  forall n1 n2,
+    simBig n1 n2 -> sim {| out := S n1 |} {| out := S n2 |}.
+Proof.
+  cofix CH.
+  intros n1 n2 H.
+  constructor; cbn.
+  destruct H as [H]; inversion H; subst.
+  - do 2 constructor.
+    rewrite <- H1, <- H2.
+    now constructor.
+  - do 2 constructor.
+    admit.
+  - admit.
+  - 
+Abort.
 
 Lemma simBig_to_sim :
   forall n m : conat, 
@@ -100,18 +164,33 @@ Lemma simBig_to_sim :
 Proof.
   cofix CH.
   intros n m H.
-  constructor.
-  destruct H as [[]].
-  - now constructor.
-  - now apply (sim_refl {| out := n0 |}).
-(*
-  - apply simBigF_sym in H.
-    apply (Build_simBig {| out := n0 |} {| out := m0 |}) in H.
-    apply CH in H. apply H.
-*)
-  - apply (CH {| out := n0 |} {| out := m0 |}).
-    constructor; cbn.
-    now apply simBigF_sym.
-  - apply (CH {| out := n1 |} {| out := n3 |}).
-    constructor; cbn.
-    now apply simBigF_trans with n2.
+  destruct H as [H].
+  dependent induction H.
+  - constructor.
+    rewrite <- x, <- x0.
+    constructor.
+  - constructor.
+    rewrite <- x, <- x0.
+    constructor.
+    apply CH.
+Abort.
+
+Lemma simBig_to_sim :
+  forall n m : conat, 
+    simBig n m -> sim n m.
+Proof.
+  intros n m H.
+  destruct H as [H].
+  remember (out n) as n' eqn: Hn'.
+  remember (out m) as m' eqn: Hm'.
+  induction H.
+  - constructor. rewrite <- Hn', <- Hm'. admit.
+  - revert n m n1 n2 Hn' Hm' H.
+    cofix CH.
+    constructor.
+    rewrite <- Hn', <- Hm'.
+    constructor.
+    eapply CH.
+Abort.
+
+End wut.
